<?xml version='1.0'?>
<!DOCTYPE rdf:RDF SYSTEM "dtd/rdf_schema.dtd" [
         <!ENTITY rdf "http://www.w3.org/1999/02/22-rdf-syntax-ns#">
         <!ENTITY rdfs "http://www.w3.org/2000/01/rdf-schema#"> 
] >

<!-- RDFS Schema of the InfraEngine Configuration -->

<rdf:RDF
  xmlns:rdf="&rdf;"
  xmlns:rdfs="&rdfs;"
  xml:base="http://www.infraengine.com/config/">

  <!-- ==================================================================== -->

  <rdfs:Class rdf:about="Config"
    rdfs:comment="Abstract superclass of configuration classes.
    General notes: pathname specifiers are pathnames that may involve
    environment variables (starting with $) and '~' (for the user's
    home directory)." />

  <!-- ==================================================================== -->

  <rdfs:Class rdf:about="GeneralConfig"
    rdfs:comment="Configuration of general aspects.">
    <rdfs:subClassOf rdf:resource="Config" />
  </rdfs:Class>

  <rdf:Property rdf:about="tmp_dir"
    rdfs:comment="Directory for temporary files.
    The value is a pathname specifier.">
    <rdfs:domain rdf:resource="GeneralConfig" />
    <rdfs:range rdf:resource="&rdfs;Literal" />
  </rdf:Property>

  <!-- ==================================================================== -->

  <rdfs:Class rdf:about="WebgetConfig"
    rdfs:comment="Configuration of the WWW client.">
    <rdfs:subClassOf rdf:resource="Config" />
  </rdfs:Class>

  <rdf:Property rdf:about="webget_client"
    rdfs:comment="Specifies the client implementation to use.
    Supported values are: wget - use the wget program;
    pce - use an internal client implementation.">
    <rdfs:domain rdf:resource="WebgetConfig" />
    <rdfs:range rdf:resource="&rdfs;Literal" />
  </rdf:Property>

  <rdf:Property rdf:about="webget_wget_parameters"
    rdfs:comment="Extra arguments submitted to the wget program.
    The value is a string.">
    <rdfs:domain rdf:resource="WebgetConfig" />
    <rdfs:range rdf:resource="&rdfs;Literal" />
  </rdf:Property>

  <!-- ==================================================================== -->

  <rdfs:Class rdf:about="WebserverConfig"
    rdfs:comment="Configuration of the WWW server.">
    <rdfs:subClassOf rdf:resource="Config" />
  </rdfs:Class>

  <rdf:Property rdf:about="webserver_password_file"
    rdfs:comment="The value is the pathname specifier of a
    password file. See the manual for more information.">
    <rdfs:domain rdf:resource="WebserverConfig" />
    <rdfs:range rdf:resource="&rdfs;Literal" />
  </rdf:Property>

  <!-- ==================================================================== -->

  <rdfs:Class rdf:about="PagesConfig"
    rdfs:comment="Configuration of presentation aspects.">
    <rdfs:subClassOf rdf:resource="Config" />
  </rdfs:Class>

  <rdf:Property rdf:about="pages_brief_comment_size"
    rdfs:comment="Approximate size of abbreviated RDF comments that
    are displayed along with objects in the RDF browser. The value is
    a number.">
    <rdfs:domain rdf:resource="PagesConfig" />
    <rdfs:range rdf:resource="&rdfs;Literal" />
  </rdf:Property>

  <rdf:Property rdf:about="pages_dotgraph_fontname"
    rdfs:comment="The fontname used by the dot program of graphviz 
    to draw graphs. The value is a string. Available fonts depend
    on the site specific configuration of graphviz.">
    <rdfs:domain rdf:resource="PagesConfig" />
    <rdfs:range rdf:resource="&rdfs;Literal" />
  </rdf:Property>

  <rdf:Property rdf:about="pages_dotgraph_fontsize"
    rdfs:comment="The fontsize used by the dot program of graphviz to
    draw graphs. The value is a number.">
    <rdfs:domain rdf:resource="PagesConfig" />
    <rdfs:range rdf:resource="&rdfs;Literal" />
  </rdf:Property>

  <!-- ==================================================================== -->

  <rdfs:Class rdf:about="PlannerConfig"
    rdfs:comment="Configuration of presentation aspects of plans.">
    <rdfs:subClassOf rdf:resource="Config" />
  </rdfs:Class>

  <rdf:Property rdf:about="planner_dotgraph_fontname"
    rdfs:comment="The fontname used by the dot program of graphviz 
    to draw graphs. The value is a string. Available fonts depend
    on the site specific configuration of graphviz.">
    <rdfs:domain rdf:resource="PlannerConfig" />
    <rdfs:range rdf:resource="&rdfs;Literal" />
  </rdf:Property>

  <rdf:Property rdf:about="planner_dotgraph_fontsize"
    rdfs:comment="The fontsize used by the dot program of graphviz to
    draw graphs. The value is a number.">
    <rdfs:domain rdf:resource="PlannerConfig" />
    <rdfs:range rdf:resource="&rdfs;Literal" />
  </rdf:Property>

</rdf:RDF>

